src/theory/tools/comp/bir_wm_instScript.sml
@@ -14,7 +14,7 @@ open bir_htTheory;
 open bin_hoare_logicSimps;
 open HolBACoreSimps;
 
-val _ = new_theory "bir_hoare_logic_test";
+val _ = new_theory "bir_wm_inst";
 
 (******************************************************************)
 (*                         DEFINITIONS                            *)
@@ -221,191 +221,6 @@ Cases_on `n` >| [
 ]
 );
 
-
-val bir_exec_to_labels_reached_ls =
-  store_thm("bir_exec_to_labels_reached_ls",
-  ``!prog ls st m m' l l' n n' n0 c_l' c_l'' st' st''.
-    (bir_exec_to_labels_n ls prog st 1 = BER_Ended l n n0 st'') ==>
-    (bir_exec_block_n prog st m = (l,n,c_l',st'')) ==>
-    (bir_exec_block_n prog st m' = (l',n',c_l'',st')) ==>
-    st'.bst_pc.bpc_label IN ls ==>
-    ~bir_state_is_terminated st'' ==>
-    m' > 0 ==>
-    ~(n' < n)``,
-
-REPEAT STRIP_TAC >>
-subgoal `m' < m` >- (
-  METIS_TAC [bir_exec_block_n_step_ls]
-) >>
-subgoal `~bir_state_is_terminated st'` >- (
-  IMP_RES_TAC bir_exec_block_n_step_ls_running
-) >>
-IMP_RES_TAC bir_exec_to_labels_n_block_n_notin_ls >>
-REV_FULL_SIMP_TAC arith_ss []
-);
-
-
-val bir_exec_to_labels_not_reached_ls =
-  store_thm("bir_exec_to_labels_not_reached_ls",
-  ``!prog ls st m m' l' l'' l''' n' n'' n''' n0 c_l' c_l'' c_l'''
-     st' st'' st'''.
-    (bir_exec_to_labels ls prog st = BER_Ended l' n' n0 st') ==>
-    (bir_exec_block_n prog st m' = (l'',n'',c_l'',st'')) ==>
-    ~bir_state_is_terminated st ==>
-    st''.bst_pc.bpc_label IN ls ==>
-    m' > 0 ==>
-    ~(n'' < n')``,
-
-REPEAT STRIP_TAC >>
-subgoal `~bir_state_is_terminated st''` >- (
-  FULL_SIMP_TAC std_ss [bir_exec_to_labels_def,
-			bir_exec_to_labels_n_def,
-			bir_exec_steps_GEN_1_EQ_Ended] >>
-  QSPECL_X_ASSUM ``!(n:num). n < n' ==> _``
-		 [`n''`] >>
-  REV_FULL_SIMP_TAC arith_ss [] >>
-  FULL_SIMP_TAC std_ss [bir_exec_block_n_EQ_THM]
-) >>
-subgoal `st''.bst_pc.bpc_label NOTIN ls \/
-         st''.bst_pc.bpc_index <> 0` >- (
-  FULL_SIMP_TAC std_ss [bir_exec_to_labels_def,
-			bir_exec_to_labels_n_def,
-			bir_exec_steps_GEN_1_EQ_Ended] >>
-  subgoal `0 < n''` >- (
-    subgoal `0 < m'` >- (
-      FULL_SIMP_TAC arith_ss []
-    ) >>
-    IMP_RES_TAC bir_exec_block_n_block_nz_init_running
-  ) >>
-  QSPECL_X_ASSUM ``!(n:num). 0 < n /\ n < n' ==> _``
-		 [`n''`] >>
-  REV_FULL_SIMP_TAC arith_ss [] >>
-  FULL_SIMP_TAC (std_ss++holBACore_ss)
-    [bir_state_COUNT_PC_def, bir_state_is_terminated_def] >>
-  FULL_SIMP_TAC std_ss [bir_exec_block_n_EQ_THM] >>
-  REV_FULL_SIMP_TAC (std_ss++holBACore_ss) [] >> (
-    FULL_SIMP_TAC std_ss []
-  )
-) >>
-Cases_on
-  `bir_exec_infinite_steps_fun_COUNT_PCs
-     (F,(\pc. pc.bpc_index = 0)) prog st n'' < m'` >- (
-  FULL_SIMP_TAC arith_ss [bir_exec_block_n_EQ_THM,
-			  bir_state_is_terminated_def] >>
-  REV_FULL_SIMP_TAC arith_ss []
-) >>
-subgoal
-  `bir_exec_infinite_steps_fun_COUNT_PCs
-     (F,(\pc. pc.bpc_index = 0)) prog st n'' = m'` >- (
-  FULL_SIMP_TAC arith_ss [bir_exec_block_n_EQ_THM]
-) >>
-subgoal `st''.bst_pc.bpc_index = 0` >- (
-  FULL_SIMP_TAC std_ss [bir_state_is_terminated_def] >>
-  subgoal
-    `bir_exec_infinite_steps_fun prog st n'' = st''` >- (
-    FULL_SIMP_TAC (std_ss++holBACore_ss)
-      [bir_exec_block_n_EQ_THM]
-  ) >>
-  FULL_SIMP_TAC (arith_ss++holBACore_ss)
-    [bir_exec_block_n_EQ_THM, bir_state_COUNT_PC_def,
-     bir_state_is_terminated_def]
-)
-);
-
-
-val bir_exec_to_labels_nz_blocks =
-  store_thm("bir_exec_to_labels_nz_blocks",
-  ``!ls prog st l m l' n c_l' st'.
-    (bir_exec_to_labels ls prog st = BER_Looping l) ==>
-    (bir_exec_block_n prog st m = (l',n,c_l',st')) ==>
-    m > 0 ==>
-    n > 0``,
-
-REPEAT STRIP_TAC >>
-FULL_SIMP_TAC std_ss [bir_exec_to_labels_def,
-		      bir_exec_to_labels_n_def,
-		      bir_exec_steps_GEN_1_EQ_Looping] >>
-subgoal `~bir_state_is_terminated st` >- (
-  QSPECL_X_ASSUM ``!n.
-                   ~bir_state_is_terminated
-                     (bir_exec_infinite_steps_fun prog st n)``
-                 [`0`] >>
-  FULL_SIMP_TAC std_ss [bir_state_is_terminated_def,
-			bir_exec_infinite_steps_fun_REWRS]
-) >>
-IMP_RES_TAC bir_exec_block_n_block_nz_init_running >>
-REV_FULL_SIMP_TAC arith_ss []
-);
-
-
-val bir_exec_to_labels_looping_not_reached_ls =
-  store_thm("bir_exec_to_labels_looping_not_reached_ls",
-  ``!ls prog st l m l' n c_l' st'.
-    (bir_exec_to_labels ls prog st = BER_Looping l) ==>
-    (bir_exec_block_n prog st m = (l',n,c_l',st')) ==>
-    0 < m ==>
-    st'.bst_pc.bpc_label NOTIN ls``,
-
-REPEAT STRIP_TAC >>
-subgoal `0 < n` >- (
-  IMP_RES_TAC bir_exec_to_labels_nz_blocks >>
-  FULL_SIMP_TAC arith_ss []
-) >>
-FULL_SIMP_TAC std_ss [bir_exec_to_labels_def,
-		      bir_exec_to_labels_n_def,
-		      bir_exec_steps_GEN_1_EQ_Looping] >>
-QSPECL_X_ASSUM ``!(n:num). (0 < n) ==> _`` [`n`] >>
-REV_FULL_SIMP_TAC arith_ss [bir_state_COUNT_PC_def] >>
-QSPECL_X_ASSUM ``!(n:num). _`` [`n`] >>
-subgoal `bir_exec_infinite_steps_fun prog st n = st'` >- (
-  FULL_SIMP_TAC std_ss [bir_exec_block_n_EQ_THM]
-) >>
-FULL_SIMP_TAC (std_ss++holBACore_ss)
-	      [bir_state_is_terminated_def] >| [
-  IMP_RES_TAC bir_exec_block_n_block_nz_final_running >>
-  REV_FULL_SIMP_TAC arith_ss [bir_state_is_terminated_def],
-
-  FULL_SIMP_TAC std_ss []
-]
-);
-
-
-val bir_exec_to_labels_term_ls =
-  store_thm("bir_exec_to_labels_term_ls",
-  ``!prog st ls m m' l' l'' l''' n' n'' n''' n0 c_l' c_l'' c_l'''
-     st' st'' st'''.
-    (bir_exec_to_labels ls prog st = BER_Ended l' n' n0 st') ==>
-    (bir_exec_block_n prog st m = (l''',n''',c_l''',st''')) ==>
-    (bir_exec_block_n prog st m' = (l'',n'',c_l'',st'')) ==>
-    (bir_exec_block_n prog st (SUC m) = (l',n',c_l',st')) ==>
-    ~bir_state_is_terminated st''' ==>
-    m' > 0 ==>
-    ~bir_state_is_terminated st'' ==>
-    st''.bst_pc.bpc_label IN ls ==>
-    bir_state_is_terminated st' ==>
-    ~(m' < (SUC m))``, 
-
-REPEAT STRIP_TAC >>
-Cases_on `n'' = n'` >- (
-  subgoal `m' >= SUC m` >- (
-    IMP_RES_TAC bir_exec_block_n_step_eq_block_gt
-  ) >>
-  FULL_SIMP_TAC arith_ss []
-) >>
-subgoal `~(n'' < n')` >- (
-  subgoal `~bir_state_is_terminated st` >- (
-    IMP_RES_TAC bir_exec_block_n_running
-  ) >>
-  IMP_RES_TAC bir_exec_to_labels_not_reached_ls
-) >>
-subgoal `n'' > n'` >- (
-  FULL_SIMP_TAC arith_ss []
-) >>
-IMP_RES_TAC bir_exec_block_n_step_ls_running >>
-REV_FULL_SIMP_TAC arith_ss []
-);
-
-
 (******************************************************************)
 (*                         MAIN PROOF                             *)
 (******************************************************************)
@@ -429,9 +244,14 @@ CASE_TAC >| [
   CASE_TAC >| [
     (* Case 1A: Ended + Final state has status Running - regular
      *          case *)
-    FULL_SIMP_TAC std_ss [bir_exec_to_labels_def] >>
-    IMP_RES_TAC bir_exec_to_labels_n_TO_bir_exec_block_n >>
-    IMP_RES_TAC bir_exec_to_labels_n_ended_running >>
+    subgoal `?m c_l'. (m > 0) /\ (bir_exec_block_n prog ms m = (l,n,c_l',b))` >- (
+      FULL_SIMP_TAC std_ss [bir_exec_to_labels_def] >>
+      IMP_RES_TAC bir_exec_to_labels_n_TO_bir_exec_block_n >>
+      Q.EXISTS_TAC `m` >>
+      Q.EXISTS_TAC `c_l'` >>
+      FULL_SIMP_TAC arith_ss []
+    ) >>
+    IMP_RES_TAC bir_exec_to_labels_ended_running >>
     rename1 `bir_exec_block_n prog st m = (l,n,c_l',b)` >>
     rename1 `bir_exec_block_n prog st m = (l,n,c_l',st'')` >>
     EQ_TAC >| [
@@ -460,8 +280,8 @@ CASE_TAC >| [
       ) >>
       FULL_SIMP_TAC std_ss
         [bir_exec_block_n_to_FUNPOW_OPT_bir_trs] >>
-      (* Finally, use bir_exec_to_labels_n_block_n_notin_ls *)
-      IMP_RES_TAC bir_exec_to_labels_n_block_n_notin_ls >>
+      (* Finally, use bir_exec_to_labels_block_n_notin_ls *)
+      IMP_RES_TAC bir_exec_to_labels_block_n_notin_ls >>
       FULL_SIMP_TAC arith_ss [],
 
       (* Case 1AII: Assuming bir_trs plays nice, show that
@@ -473,7 +293,7 @@ CASE_TAC >| [
       rename1 `bir_exec_block_n prog st m' = (l',n',c_l'',ms')` >>
       rename1 `bir_exec_block_n prog st m' = (l',n',c_l'',st')` >>
       (* Prove that n = n' using the original hypothesis of the
-       * goal*)
+       * goal *)
       subgoal `n = n'` >- (
 	subgoal `~(n' < n)` >- (
 	  IMP_RES_TAC bir_exec_to_labels_reached_ls
